Fixed some formatting inconsistencies

Sequences/SeqExtrema.dfy
@@ -1,43 +1,59 @@
 include "SeqLast.dfy"
-include "Mathematics.dfy"
+include "../Mathematics.dfy"
 
 module SeqExtrema {
 
   import opened SeqLast
   import Math = Mathematics
 
-  // returns the maximum integer value in the sequence
+  /* returns the maximum integer value in the sequence */
   function method {:opaque} max(s: seq<int>): int
     requires 0 < |s|
     ensures forall k :: k in s ==> max(s) >= k
     ensures max(s) in s
   {
-    assert s == drop_last(s) + [last(s)];
-
-    if |s| == 1 then s[0] else Math.max(max(drop_last(s)), last(s))
+    assert s == [s[0]] + s[1..];
+    if |s| == 1 then s[0] else Math.max(s[0], max(s[1..]))
   }
 
-  // function method max_of_concat(a: seq<int>, b: seq<int>): int
-  //   requires 0 < |a| && 0 < |b|
-  //   ensures max(a+b) >= max(a)
-  //   ensures max(a+b) >= max(b)
-  //   ensures forall i :: i in a+b ==> max(a+b) >= i
-  // {
-  //   reveal_max();
-  //   if max(b) >= max(a) then max(b) else max(a)
-  // }
+  lemma lemma_max_of_concat(a: seq<int>, b: seq<int>)
+    requires 0 < |a| && 0 < |b|
+    ensures max(a+b) >= max(a)
+    ensures max(a+b) >= max(b)
+    ensures forall i :: i in a+b ==> max(a+b) >= i
+  {
+    reveal_max();
+    if |a| == 1 {
+    } else {
+      assert a[1..] + b == (a + b)[1..];
+      lemma_max_of_concat(a[1..], b);
+    }
+  }
 
-  // returns the minimum integer value in the sequence
+  /* returns the minimum integer value in the sequence */
   function method {:opaque} min(s: seq<int>): int
     requires 0 < |s|
     ensures forall k :: k in s ==> min(s) <= k
     ensures min(s) in s
   {
-    assert s == drop_last(s) + [last(s)];
-    if |s| == 1 then s[0] else Math.min(min(drop_last(s)), last(s))
+    assert s == [s[0]] + s[1..];
+    if |s| == 1 then s[0] else Math.min(s[0], min(s[1..]))
   }
 
-  // necessary for lemma_subseq_max
+   lemma lemma_min_of_concat(a: seq<int>, b: seq<int>)
+    requires 0 < |a| && 0 < |b|
+    ensures min(a+b) <= min(a)
+    ensures min(a+b) <= min(b)
+    ensures forall i :: i  in a+b ==> min(a+b) <= i
+  {
+    reveal_min();
+    if |a| == 1 {
+    } else {
+      assert a[1..] + b == (a + b)[1..];
+      lemma_min_of_concat(a[1..], b);
+    }
+  }
+
   /* the maximum value in sequence 1 is greater than or equal to the maximum
   value of sequence 2 */
   lemma lemma_max_correspondence(s1:seq<int>, s2:seq<int>, wit: seq<nat>)
@@ -55,8 +71,8 @@ module SeqExtrema {
     }
   }
 
-  /* the maximum element in any subsequence will not be 
-  greater than the maximum element in the full sequence */
+  /* the maximum element in any subsequence will not be greater than the maximum element in 
+  the full sequence */
   lemma lemma_subseq_max(s: seq<int>, from: nat, to: nat)
     requires from < to <= |s|
     ensures max(s[from .. to]) <= max(s)
@@ -82,8 +98,9 @@ module SeqExtrema {
   lemma lemma_subseq_min(s: seq<int>, from: nat, to: nat)
     requires from < to <= |s|
     ensures min(s[from..to]) >= min(s)
-    {
-      var subseq := s[from..to];
-      lemma_min_correspondence(s, subseq, seq(|subseq|, i requires 0<=i<|subseq| => i + from));
-    }
+  {
+    var subseq := s[from..to];
+    lemma_min_correspondence(s, subseq, seq(|subseq|, i requires 0<=i<|subseq| => i + from));
+  }
+
 }
