NativeTypes.dfy
@@ -1,0 +1,13 @@
+module NativeTypes {
+
+  newtype uint8 =  x | 0 <= x < 0x100
+  newtype uint16 = x | 0 <= x < 0x1_0000
+  newtype uint32 = x | 0 <= x < 0x1_0000_0000
+  newtype uint64 = x | 0 <= x < 0x1_0000_0000_0000_0000
+
+  newtype int8  = x | -0x80 <= x < 0x80
+  newtype int16 = x | -0x8000 <= x < 0x80000
+  newtype int32 = x | -0x8000_0000 <= x < 0x8000_0000
+  newtype int64 = x | -0x8000_0000_0000_0000 <= x < 0x8000_0000_0000_0000
+  
+}
