Options.dfy
@@ -1,14 +1,5 @@
-module {:extern} Options {
-  newtype uint8 =  x | 0 <= x < 0x100
-  newtype uint16 = x | 0 <= x < 0x1_0000
-  newtype uint32 = x | 0 <= x < 0x1_0000_0000
-  newtype uint64 = x | 0 <= x < 0x1_0000_0000_0000_0000
-
-  newtype int8  = x | -0x80 <= x < 0x80
-  newtype int16 = x | -0x8000 <= x < 0x80000
-  newtype int32 = x | -0x8000_0000 <= x < 0x8000_0000
-  newtype int64 = x | -0x8000_0000_0000_0000 <= x < 0x8000_0000_0000_0000
-
+module Options {
+  
   datatype Option<T> = None | Some(value: T) {
     function method to_result(): Result<T> {
       match this
