Sequences/SeqHigherLevel.dfy
@@ -1,16 +1,17 @@
 module SeqHigherLevel { 
-  // applies a transformation function on the sequence
-  function method {:opaque} Map<T,R>(f: (T ~> R), s: seq<T>): (result: seq<R>)
+
+  /* applies a transformation function on the sequence; this acts as "map" in other languages */
+  function method {:opaque} apply<T,R>(f: (T ~> R), s: seq<T>): (result: seq<R>)
     requires forall i :: 0 <= i < |s| ==> f.requires(s[i])
     ensures |result| == |s|
     ensures forall i :: 0 <= i < |s| ==> result[i] == f(s[i]);
     reads set i, o | 0 <= i < |s| && o in f.reads(s[i]):: o
   {
     if |s| == 0 then []
-    else  [f(s[0])] + Map(f, s[1..])
+    else  [f(s[0])] + apply(f, s[1..])
   }
 
-  // uses a selection function to select elements from the sequence
+  /* uses a selection function to select elements from the sequence */
   function method {:opaque} filter<T>(f : (T ~> bool), s: seq<T>): (result: seq<T>)
     requires forall i :: 0 <= i < |s| ==> f.requires(s[i])
     ensures |result| <= |s|
@@ -32,4 +33,5 @@ module SeqHigherLevel {
     if |s| == 0 then init
     else f(fold_right(f, init, s[1..]), s[0])
   }
+
 }
